module plfa.part1.Induction where


import Relation.Binary.PropositionalEquality as Eq
open Eq using (_≡_; refl; cong; sym; trans)
open Eq.≡-Reasoning using (begin_; _≡⟨⟩_; _∎)
open import Data.Nat using (ℕ; zero; suc; _+_; _*_; _∸_)

+-assoc : ∀ (m n p : ℕ) → (m + n) + p ≡ m + (n + p)
+-assoc zero n p = refl
+-assoc (suc m) n p rewrite +-assoc m n p = refl

+-identityʳ : ∀ (m : ℕ) → m + zero ≡ m
+-identityʳ zero = refl
+-identityʳ (suc m) rewrite +-identityʳ m = refl

+-suc : ∀ (m n : ℕ) → m + suc n ≡ suc (m + n)
+-suc zero n = refl
+-suc (suc m) n rewrite +-suc m n = refl


+-comm : ∀ (m n : ℕ) → m + n ≡ n + m
+-comm zero n rewrite +-identityʳ n = refl
+-comm (suc m) n rewrite +-suc n m | +-comm m n = refl


+-swap : ∀ (m n p : ℕ) → m + (n + p) ≡ n + (m + p)
+-swap m n p rewrite sym (+-assoc m n p) | +-comm m n | +-assoc n m p = refl

*-distrib-+ : ∀ (m n p : ℕ) → (m + n) * p ≡ m * p + n * p
*-distrib-+ zero n p = refl
*-distrib-+ (suc m) n p rewrite *-distrib-+ m n p | +-assoc p (m * p) (n * p)= refl
 

*-assoc : ∀ (m n p : ℕ) → (m * n) * p ≡ m * (n * p)
*-assoc zero n p = refl
*-assoc (suc m) n p rewrite *-assoc m n p | *-distrib-+ n (m * n) p | sym (*-assoc m n p) = refl

*-identityʳ : ∀ (m : ℕ) → m * zero ≡ zero
*-identityʳ zero = refl
*-identityʳ (suc m) rewrite *-identityʳ m = refl

*-suc : ∀ (m n : ℕ) → m * suc n ≡ (m * n) + m
*-suc zero n = refl
*-suc (suc m) n rewrite *-suc m n | +-assoc n (m * n) (suc m) | +-suc (m * n) m | +-suc n (m * n + m)= refl

*-comm : ∀ (m n : ℕ) → m * n ≡ n * m
*-comm zero n rewrite *-identityʳ n = refl
*-comm (suc m) n rewrite *-comm m n | *-suc n m | +-comm n (n * m)= refl
